IterM

src/Init/Data/Iterators/Combinators/Monadic/FlatMap.lean
@@ -47,12 +47,24 @@ def IterM.flattenAfter {α α₂ β : Type w} {m : Type w → Type w'} [Monad m]
   (toIterM (α := Flatten α α₂ β m) ⟨it₁, it₂⟩ m β : IterM m β)
 
 @[always_inline]
+public def IterM.flatMapAfterM {α : Type w} {β : Type w} {α₂ : Type w}
+    {γ : Type w} {m : Type w → Type w'} [Monad m] [Iterator α m β] [Iterator α₂ m γ]
+    (f : β → m (IterM (α := α₂) m γ)) (it₁ : IterM (α := α) m β) (it₂ : Option (IterM (α := α₂) m γ)) :=
+  ((it₁.mapM f).flattenAfter it₂ : IterM m γ)
+
+@[always_inline, expose]
+public def IterM.flatMapM {α : Type w} {β : Type w} {α₂ : Type w}
+    {γ : Type w} {m : Type w → Type w'} [Monad m] [Iterator α m β] [Iterator α₂ m γ]
+    (f : β → m (IterM (α := α₂) m γ)) (it : IterM (α := α) m β) :=
+  (it.flatMapAfterM f none : IterM m γ)
+
+@[always_inline]
 public def IterM.flatMapAfter {α : Type w} {β : Type w} {α₂ : Type w}
     {γ : Type w} {m : Type w → Type w'} [Monad m] [Iterator α m β] [Iterator α₂ m γ]
     (f : β → IterM (α := α₂) m γ) (it₁ : IterM (α := α) m β) (it₂ : Option (IterM (α := α₂) m γ)) :=
   ((it₁.map f).flattenAfter it₂ : IterM m γ)
 
-@[always_inline]
+@[always_inline, expose]
 public def IterM.flatMap {α : Type w} {β : Type w} {α₂ : Type w}
     {γ : Type w} {m : Type w → Type w'} [Monad m] [Iterator α m β] [Iterator α₂ m γ]
     (f : β → IterM (α := α₂) m γ) (it : IterM (α := α) m β) :=
