src/Init/Data/Iterators/Lemmas/Combinators/Monadic/FlatMap.lean
@@ -1,0 +1,345 @@
+/-
+Copyright (c) 2025 Lean FRO, LLC. All rights reserved.
+Released under Apache 2.0 license as described in the file LICENSE.
+Authors: Paul Reichert
+-/
+module
+
+prelude
+public import Init.Data.Iterators.Internal.LawfulMonadLiftFunction
+public import Init.Data.Iterators.Combinators.Monadic.FlatMap
+import all Init.Data.Iterators.Combinators.Monadic.FlatMap
+public import Init.Data.Iterators.Lemmas.Consumers.Monadic
+public import Init.Data.Iterators.Consumers.Monadic.Collect
+import all Init.Data.Iterators.Consumers.Monadic.Collect
+import Init.Data.Iterators.Lemmas.Combinators.Monadic.FilterMap
+
+namespace Std.Iterators
+open Std.Internal
+
+theorem IterM.step_flattenAfter {α α₂ β : Type w} {m : Type w → Type w'} [Monad m]
+    [Iterator α m (IterM (α := α₂) m β)] [Iterator α₂ m β]
+    {it₁ : IterM (α := α) m (IterM (α := α₂) m β)} {it₂ : Option (IterM (α := α₂) m β)} :
+  (it₁.flattenAfter it₂).step = (do
+    match it₂ with
+    | none =>
+      match ← it₁.step with
+      | .yield it₁' it₂' h => return .skip (it₁'.flattenAfter (some it₂')) (.outerYield h)
+      | .skip it₁' h => return .skip (it₁'.flattenAfter none) (.outerSkip h)
+      | .done h => return .done (.outerDone h)
+    | some it₂ =>
+      match ← it₂.step with
+      | .yield it₂' out h => return .yield (it₁.flattenAfter (some it₂')) out (.innerYield h)
+      | .skip it₂' h => return .skip (it₁.flattenAfter (some it₂')) (.innerSkip h)
+      | .done h => return .skip (it₁.flattenAfter none) (.innerDone h)) := by
+  cases it₂
+  all_goals
+  · apply bind_congr; intro step
+    split <;> simp [IterM.flattenAfter, toIterM]
+
+public theorem Flatten.IsPlausibleStep.outerYield_flatMapM {α : Type w} {β : Type w} {α₂ : Type w}
+    {γ : Type w} {m : Type w → Type w'} [Monad m] [LawfulMonad m] [Iterator α m β] [Iterator α₂ m γ]
+    {f : β → m (IterM (α := α₂) m γ)} {it₁ it₁' : IterM (α := α) m β} {it₂' b}
+    (h : it₁.IsPlausibleStep (.yield it₁' b)) :
+    (it₁.flatMapAfterM f none).IsPlausibleStep (.skip (it₁'.flatMapAfterM f (some it₂'))) :=
+  .outerYield (.yieldSome h ⟨⟨_, trivial⟩, rfl⟩)
+
+public theorem Flatten.IsPlausibleStep.outerSkip_flatMapM {α : Type w} {β : Type w} {α₂ : Type w}
+    {γ : Type w} {m : Type w → Type w'} [Monad m] [LawfulMonad m] [Iterator α m β] [Iterator α₂ m γ]
+    {f : β → m (IterM (α := α₂) m γ)} {it₁ it₁' : IterM (α := α) m β}
+    (h : it₁.IsPlausibleStep (.skip it₁')) :
+    (it₁.flatMapAfterM f none).IsPlausibleStep (.skip (it₁'.flatMapAfterM f none)) :=
+  .outerSkip (.skip h)
+
+public theorem Flatten.IsPlausibleStep.outerDone_flatMapM {α : Type w} {β : Type w} {α₂ : Type w}
+    {γ : Type w} {m : Type w → Type w'} [Monad m] [LawfulMonad m] [Iterator α m β] [Iterator α₂ m γ]
+    {f : β → m (IterM (α := α₂) m γ)} {it₁ : IterM (α := α) m β}
+    (h : it₁.IsPlausibleStep .done) :
+    (it₁.flatMapAfterM f none).IsPlausibleStep .done :=
+  .outerDone (.done h)
+
+public theorem Flatten.IsPlausibleStep.innerYield_flatMapM {α : Type w} {β : Type w} {α₂ : Type w}
+    {γ : Type w} {m : Type w → Type w'} [Monad m] [LawfulMonad m] [Iterator α m β] [Iterator α₂ m γ]
+    {f : β → m (IterM (α := α₂) m γ)} {it₁ : IterM (α := α) m β} {it₂ it₂' b}
+    (h : it₂.IsPlausibleStep (.yield it₂' b)) :
+    (it₁.flatMapAfterM f (some it₂)).IsPlausibleStep (.yield (it₁.flatMapAfterM f (some it₂')) b) :=
+  .innerYield h
+
+public theorem Flatten.IsPlausibleStep.innerSkip_flatMapM {α : Type w} {β : Type w} {α₂ : Type w}
+    {γ : Type w} {m : Type w → Type w'} [Monad m] [LawfulMonad m] [Iterator α m β] [Iterator α₂ m γ]
+    {f : β → m (IterM (α := α₂) m γ)} {it₁ : IterM (α := α) m β} {it₂ it₂'}
+    (h : it₂.IsPlausibleStep (.skip it₂')) :
+    (it₁.flatMapAfterM f (some it₂)).IsPlausibleStep (.skip (it₁.flatMapAfterM f (some it₂'))) :=
+  .innerSkip h
+
+public theorem Flatten.IsPlausibleStep.innerDone_flatMapM {α : Type w} {β : Type w} {α₂ : Type w}
+    {γ : Type w} {m : Type w → Type w'} [Monad m] [LawfulMonad m] [Iterator α m β] [Iterator α₂ m γ]
+    {f : β → m (IterM (α := α₂) m γ)} {it₁ : IterM (α := α) m β} {it₂}
+    (h : it₂.IsPlausibleStep .done) :
+    (it₁.flatMapAfterM f (some it₂)).IsPlausibleStep (.skip (it₁.flatMapAfterM f none)) :=
+  .innerDone h
+
+public theorem Flatten.IsPlausibleStep.outerYield_flatMap {α : Type w} {β : Type w} {α₂ : Type w}
+    {γ : Type w} {m : Type w → Type w'} [Monad m] [LawfulMonad m] [Iterator α m β] [Iterator α₂ m γ]
+    {f : β → IterM (α := α₂) m γ} {it₁ it₁' : IterM (α := α) m β} {b}
+    (h : it₁.IsPlausibleStep (.yield it₁' b)) :
+    (it₁.flatMapAfter f none).IsPlausibleStep (.skip (it₁'.flatMapAfter f (some (f b)))) :=
+  .outerYield (.yieldSome h ⟨⟨_, rfl⟩, rfl⟩)
+
+public theorem Flatten.IsPlausibleStep.outerSkip_flatMap {α : Type w} {β : Type w} {α₂ : Type w}
+    {γ : Type w} {m : Type w → Type w'} [Monad m] [LawfulMonad m] [Iterator α m β] [Iterator α₂ m γ]
+    {f : β → IterM (α := α₂) m γ} {it₁ it₁' : IterM (α := α) m β}
+    (h : it₁.IsPlausibleStep (.skip it₁')) :
+    (it₁.flatMapAfter f none).IsPlausibleStep (.skip (it₁'.flatMapAfter f none)) :=
+  .outerSkip (.skip h)
+
+public theorem Flatten.IsPlausibleStep.outerDone_flatMap {α : Type w} {β : Type w} {α₂ : Type w}
+    {γ : Type w} {m : Type w → Type w'} [Monad m] [LawfulMonad m] [Iterator α m β] [Iterator α₂ m γ]
+    {f : β → IterM (α := α₂) m γ} {it₁ : IterM (α := α) m β}
+    (h : it₁.IsPlausibleStep .done) :
+    (it₁.flatMapAfter f none).IsPlausibleStep .done :=
+  .outerDone (.done h)
+
+public theorem Flatten.IsPlausibleStep.innerYield_flatMap {α : Type w} {β : Type w} {α₂ : Type w}
+    {γ : Type w} {m : Type w → Type w'} [Monad m] [LawfulMonad m] [Iterator α m β] [Iterator α₂ m γ]
+    {f : β → IterM (α := α₂) m γ} {it₁ : IterM (α := α) m β} {it₂ it₂' b}
+    (h : it₂.IsPlausibleStep (.yield it₂' b)) :
+    (it₁.flatMapAfter f (some it₂)).IsPlausibleStep (.yield (it₁.flatMapAfter f (some it₂')) b) :=
+  .innerYield h
+
+public theorem Flatten.IsPlausibleStep.innerSkip_flatMap {α : Type w} {β : Type w} {α₂ : Type w}
+    {γ : Type w} {m : Type w → Type w'} [Monad m] [LawfulMonad m] [Iterator α m β] [Iterator α₂ m γ]
+    {f : β → IterM (α := α₂) m γ} {it₁ : IterM (α := α) m β} {it₂ it₂'}
+    (h : it₂.IsPlausibleStep (.skip it₂')) :
+    (it₁.flatMapAfter f (some it₂)).IsPlausibleStep (.skip (it₁.flatMapAfter f (some it₂'))) :=
+  .innerSkip h
+
+public theorem Flatten.IsPlausibleStep.innerDone_flatMap {α : Type w} {β : Type w} {α₂ : Type w}
+    {γ : Type w} {m : Type w → Type w'} [Monad m] [LawfulMonad m] [Iterator α m β] [Iterator α₂ m γ]
+    {f : β → IterM (α := α₂) m γ} {it₁ : IterM (α := α) m β} {it₂}
+    (h : it₂.IsPlausibleStep .done) :
+    (it₁.flatMapAfter f (some it₂)).IsPlausibleStep (.skip (it₁.flatMapAfter f none)) :=
+  .innerDone h
+
+public theorem IterM.step_flatMapAfterM {α : Type w} {β : Type w} {α₂ : Type w}
+    {γ : Type w} {m : Type w → Type w'} [Monad m] [LawfulMonad m] [Iterator α m β] [Iterator α₂ m γ]
+    {f : β → m (IterM (α := α₂) m γ)} {it₁ : IterM (α := α) m β} {it₂ : Option (IterM (α := α₂) m γ)} :
+  (it₁.flatMapAfterM f it₂).step = (do
+    match it₂ with
+    | none =>
+      match ← it₁.step with
+      | .yield it₁' b h =>
+        return .skip (it₁'.flatMapAfterM f (some (← f b))) (.outerYield_flatMapM h)
+      | .skip it₁' h => return .skip (it₁'.flatMapAfterM f none) (.outerSkip_flatMapM h)
+      | .done h => return .done (.outerDone_flatMapM h)
+    | some it₂ =>
+      match ← it₂.step with
+      | .yield it₂' out h => return .yield (it₁.flatMapAfterM f (some it₂')) out (.innerYield_flatMapM h)
+      | .skip it₂' h => return .skip (it₁.flatMapAfterM f (some it₂')) (.innerSkip_flatMapM h)
+      | .done h => return .skip (it₁.flatMapAfterM f none) (.innerDone_flatMapM h)) := by
+  simp only [flatMapAfterM, step_flattenAfter, IterM.step_mapM]
+  split
+  · simp only [bind_assoc]
+    apply bind_congr; intro step
+    split <;> simp
+  · rfl
+
+public theorem IterM.step_flatMapM {α : Type w} {β : Type w} {α₂ : Type w}
+    {γ : Type w} {m : Type w → Type w'} [Monad m] [LawfulMonad m] [Iterator α m β] [Iterator α₂ m γ]
+    {f : β → m (IterM (α := α₂) m γ)} {it₁ : IterM (α := α) m β} :
+  (it₁.flatMapM f).step = (do
+    match ← it₁.step with
+    | .yield it₁' b h =>
+      return .skip (it₁'.flatMapAfterM f (some (← f b)))
+        (.outerYield_flatMapM h)
+    | .skip it₁' h => return .skip (it₁'.flatMapAfterM f none) (.outerSkip_flatMapM h)
+    | .done h => return .done (.outerDone_flatMapM h)) := by
+  simp [flatMapM, step_flatMapAfterM]
+
+public theorem IterM.step_flatMapAfter {α : Type w} {β : Type w} {α₂ : Type w}
+    {γ : Type w} {m : Type w → Type w'} [Monad m] [LawfulMonad m] [Iterator α m β] [Iterator α₂ m γ]
+    {f : β → IterM (α := α₂) m γ} {it₁ : IterM (α := α) m β} {it₂ : Option (IterM (α := α₂) m γ)} :
+  (it₁.flatMapAfter f it₂).step = (do
+    match it₂ with
+    | none =>
+      match ← it₁.step with
+      | .yield it₁' b h =>
+        return .skip (it₁'.flatMapAfter f (some (f b))) (.outerYield_flatMap h)
+      | .skip it₁' h => return .skip (it₁'.flatMapAfter f none) (.outerSkip_flatMap h)
+      | .done h => return .done (.outerDone_flatMap h)
+    | some it₂ =>
+      match ← it₂.step with
+      | .yield it₂' out h => return .yield (it₁.flatMapAfter f (some it₂')) out (.innerYield_flatMap h)
+      | .skip it₂' h => return .skip (it₁.flatMapAfter f (some it₂')) (.innerSkip_flatMap h)
+      | .done h => return .skip (it₁.flatMapAfter f none) (.innerDone_flatMap h)) := by
+  simp only [flatMapAfter, step_flattenAfter, IterM.step_map]
+  split
+  · simp only [bind_assoc]
+    apply bind_congr; intro step
+    split <;> simp
+  · rfl
+
+public theorem IterM.step_flatMap {α : Type w} {β : Type w} {α₂ : Type w}
+    {γ : Type w} {m : Type w → Type w'} [Monad m] [LawfulMonad m] [Iterator α m β] [Iterator α₂ m γ]
+    {f : β → IterM (α := α₂) m γ} {it₁ : IterM (α := α) m β} :
+  (it₁.flatMap f).step = (do
+    match ← it₁.step with
+    | .yield it₁' b h =>
+      return .skip (it₁'.flatMapAfter f (some (f b))) (.outerYield_flatMap h)
+    | .skip it₁' h => return .skip (it₁'.flatMapAfter f none) (.outerSkip_flatMap h)
+    | .done h => return .done (.outerDone_flatMap h)) := by
+  simp [flatMap, step_flatMapAfter]
+
+theorem IterM.toList_flattenAfter {α α₂ β : Type w} {m : Type w → Type w'} [Monad m] [LawfulMonad m]
+    [Iterator α m (IterM (α := α₂) m β)] [Iterator α₂ m β] [Finite α m] [Finite α₂ m]
+    [IteratorCollect α m m] [IteratorCollect α₂ m m]
+    [LawfulIteratorCollect α m m] [LawfulIteratorCollect α₂ m m]
+    {it₁ : IterM (α := α) m (IterM (α := α₂) m β)} {it₂ : Option (IterM (α := α₂) m β)} :
+    (it₁.flattenAfter it₂).toList = do
+      match it₂ with
+      | none => List.flatten <$> (it₁.mapM fun it₂ => it₂.toList).toList
+      | some it₂ => return (← it₂.toList) ++ (← List.flatten <$> (it₁.mapM fun it₂ => it₂.toList).toList) := by
+  induction it₁ using IterM.inductSteps generalizing it₂ with | step it₁ ihy₁ ihs₁ =>
+  have hn : (it₁.flattenAfter none).toList =
+      List.flatten <$> (it₁.mapM fun it₂ => it₂.toList).toList := by
+    rw [toList_eq_match_step, toList_eq_match_step, step_flattenAfter, step_mapM]
+    simp only [bind_assoc, map_eq_pure_bind]
+    apply bind_congr; intro step
+    split
+    · simp [ihy₁ ‹_›]
+    · simp [ihs₁ ‹_›]
+    · simp
+  cases it₂
+  · exact hn
+  · rename_i ih₂
+    induction ih₂ using IterM.inductSteps with | step it₂ ihy₂ ihs₂ =>
+    rw [toList_eq_match_step, step_flattenAfter, bind_assoc]
+    simp only
+    rw [toList_eq_match_step, bind_assoc]
+    apply bind_congr; intro step
+    cases step using PlausibleIterStep.casesOn
+    · simp [ihy₂ ‹_›]
+    · simp [ihs₂ ‹_›]
+    · simp [hn]
+
+theorem IterM.toArray_flattenAfter {α α₂ β : Type w} {m : Type w → Type w'} [Monad m] [LawfulMonad m]
+    [Iterator α m (IterM (α := α₂) m β)] [Iterator α₂ m β] [Finite α m] [Finite α₂ m]
+    [IteratorCollect α m m] [IteratorCollect α₂ m m]
+    [LawfulIteratorCollect α m m] [LawfulIteratorCollect α₂ m m]
+    {it₁ : IterM (α := α) m (IterM (α := α₂) m β)} {it₂ : Option (IterM (α := α₂) m β)} :
+    (it₁.flattenAfter it₂).toArray = do
+      match it₂ with
+      | none => Array.flatten <$> (it₁.mapM fun it₂ => it₂.toArray).toArray
+      | some it₂ => return (← it₂.toArray) ++ (← Array.flatten <$> (it₁.mapM fun it₂ => it₂.toArray).toArray) := by
+  induction it₁ using IterM.inductSteps generalizing it₂ with | step it₁ ihy₁ ihs₁ =>
+  have hn : (it₁.flattenAfter none).toArray =
+      Array.flatten <$> (it₁.mapM fun it₂ => it₂.toArray).toArray := by
+    rw [toArray_eq_match_step, toArray_eq_match_step, step_flattenAfter, step_mapM]
+    simp only [bind_assoc, map_eq_pure_bind]
+    apply bind_congr; intro step
+    split
+    · simp [ihy₁ ‹_›]
+    · simp [ihs₁ ‹_›]
+    · simp
+  cases it₂
+  · exact hn
+  · rename_i ih₂
+    induction ih₂ using IterM.inductSteps with | step it₂ ihy₂ ihs₂ =>
+    rw [toArray_eq_match_step, step_flattenAfter, bind_assoc]
+    simp only
+    rw [toArray_eq_match_step, bind_assoc]
+    apply bind_congr; intro step
+    cases step using PlausibleIterStep.casesOn
+    · simp [ihy₂ ‹_›]
+    · simp [ihs₂ ‹_›]
+    · simp [hn]
+
+public theorem IterM.toList_flatMapAfterM {α α₂ β γ : Type w} {m : Type w → Type w'} [Monad m]
+    [LawfulMonad m] [Iterator α m β] [Iterator α₂ m γ] [Finite α m] [Finite α₂ m]
+    [IteratorCollect α m m] [IteratorCollect α₂ m m]
+    [LawfulIteratorCollect α m m] [LawfulIteratorCollect α₂ m m]
+    {f : β → m (IterM (α := α₂) m γ)}
+    {it₁ : IterM (α := α) m β} {it₂ : Option (IterM (α := α₂) m γ)} :
+    (it₁.flatMapAfterM f it₂).toList = do
+      match it₂ with
+      | none => List.flatten <$> (it₁.mapM fun b => do (← f b).toList).toList
+      | some it₂ => return (← it₂.toList) ++
+          (← List.flatten <$> (it₁.mapM fun b => do (← f b).toList).toList) := by
+  simp [flatMapAfterM, toList_flattenAfter]; rfl
+
+public theorem IterM.toArray_flatMapAfterM {α α₂ β γ : Type w} {m : Type w → Type w'} [Monad m]
+    [LawfulMonad m] [Iterator α m β] [Iterator α₂ m γ] [Finite α m] [Finite α₂ m]
+    [IteratorCollect α m m] [IteratorCollect α₂ m m]
+    [LawfulIteratorCollect α m m] [LawfulIteratorCollect α₂ m m]
+    {f : β → m (IterM (α := α₂) m γ)}
+    {it₁ : IterM (α := α) m β} {it₂ : Option (IterM (α := α₂) m γ)} :
+    (it₁.flatMapAfterM f it₂).toArray = do
+      match it₂ with
+      | none => Array.flatten <$> (it₁.mapM fun b => do (← f b).toArray).toArray
+      | some it₂ => return (← it₂.toArray) ++
+          (← Array.flatten <$> (it₁.mapM fun b => do (← f b).toArray).toArray) := by
+  simp [flatMapAfterM, toArray_flattenAfter]; rfl
+
+public theorem IterM.toList_flatMapM {α α₂ β γ : Type w} {m : Type w → Type w'} [Monad m]
+    [LawfulMonad m] [Iterator α m β] [Iterator α₂ m γ] [Finite α m] [Finite α₂ m]
+    [IteratorCollect α m m] [IteratorCollect α₂ m m]
+    [LawfulIteratorCollect α m m] [LawfulIteratorCollect α₂ m m]
+    {f : β → m (IterM (α := α₂) m γ)}
+    {it₁ : IterM (α := α) m β} :
+    (it₁.flatMapM f).toList = List.flatten <$> (it₁.mapM fun b => do (← f b).toList).toList := by
+  simp [flatMapM, toList_flatMapAfterM]
+
+public theorem IterM.toArray_flatMapM {α α₂ β γ : Type w} {m : Type w → Type w'} [Monad m]
+    [LawfulMonad m] [Iterator α m β] [Iterator α₂ m γ] [Finite α m] [Finite α₂ m]
+    [IteratorCollect α m m] [IteratorCollect α₂ m m]
+    [LawfulIteratorCollect α m m] [LawfulIteratorCollect α₂ m m]
+    {f : β → m (IterM (α := α₂) m γ)}
+    {it₁ : IterM (α := α) m β} :
+    (it₁.flatMapM f).toArray = Array.flatten <$> (it₁.mapM fun b => do (← f b).toArray).toArray := by
+  simp [flatMapM, toArray_flatMapAfterM]
+
+public theorem IterM.toList_flatMapAfter {α α₂ β γ : Type w} {m : Type w → Type w'} [Monad m]
+    [LawfulMonad m] [Iterator α m β] [Iterator α₂ m γ] [Finite α m] [Finite α₂ m]
+    [IteratorCollect α m m] [IteratorCollect α₂ m m]
+    [LawfulIteratorCollect α m m] [LawfulIteratorCollect α₂ m m]
+    {f : β → IterM (α := α₂) m γ}
+    {it₁ : IterM (α := α) m β} {it₂ : Option (IterM (α := α₂) m γ)} :
+    (it₁.flatMapAfter f it₂).toList = do
+      match it₂ with
+      | none => List.flatten <$> (it₁.mapM fun b => (f b).toList).toList
+      | some it₂ => return (← it₂.toList) ++
+          (← List.flatten <$> (it₁.mapM fun b => (f b).toList).toList) := by
+  simp [flatMapAfter, toList_flattenAfter]; rfl
+
+public theorem IterM.toArray_flatMapAfter {α α₂ β γ : Type w} {m : Type w → Type w'} [Monad m]
+    [LawfulMonad m] [Iterator α m β] [Iterator α₂ m γ] [Finite α m] [Finite α₂ m]
+    [IteratorCollect α m m] [IteratorCollect α₂ m m]
+    [LawfulIteratorCollect α m m] [LawfulIteratorCollect α₂ m m]
+    {f : β → IterM (α := α₂) m γ}
+    {it₁ : IterM (α := α) m β} {it₂ : Option (IterM (α := α₂) m γ)} :
+    (it₁.flatMapAfter f it₂).toArray = do
+      match it₂ with
+      | none => Array.flatten <$> (it₁.mapM fun b => (f b).toArray).toArray
+      | some it₂ => return (← it₂.toArray) ++
+          (← Array.flatten <$> (it₁.mapM fun b => (f b).toArray).toArray) := by
+  simp [flatMapAfter, toArray_flattenAfter]; rfl
+
+public theorem IterM.toList_flatMap {α α₂ β γ : Type w} {m : Type w → Type w'} [Monad m]
+    [LawfulMonad m] [Iterator α m β] [Iterator α₂ m γ] [Finite α m] [Finite α₂ m]
+    [Iterator α m β] [Iterator α₂ m γ] [Finite α m] [Finite α₂ m]
+    [IteratorCollect α m m] [IteratorCollect α₂ m m]
+    [LawfulIteratorCollect α m m] [LawfulIteratorCollect α₂ m m]
+    {f : β → IterM (α := α₂) m γ}
+    {it₁ : IterM (α := α) m β} :
+    (it₁.flatMap f).toList = List.flatten <$> (it₁.mapM fun b => (f b).toList).toList := by
+  simp [flatMap, toList_flatMapAfter]
+
+public theorem IterM.toArray_flatMap {α α₂ β γ : Type w} {m : Type w → Type w'} [Monad m]
+    [LawfulMonad m] [Iterator α m β] [Iterator α₂ m γ] [Finite α m] [Finite α₂ m]
+    [Iterator α m β] [Iterator α₂ m γ] [Finite α m] [Finite α₂ m]
+    [IteratorCollect α m m] [IteratorCollect α₂ m m]
+    [LawfulIteratorCollect α m m] [LawfulIteratorCollect α₂ m m]
+    {f : β → IterM (α := α₂) m γ}
+    {it₁ : IterM (α := α) m β} :
+    (it₁.flatMap f).toArray = Array.flatten <$> (it₁.mapM fun b => (f b).toArray).toArray := by
+  simp [flatMap, toArray_flatMapAfter]
